weird implementation of ZFC

FormalizationOfMyUniversityMathematics/ElemMath/Definition_14_1.lean
@@ -1,42 +1,101 @@
+class SetNotation (set : Type u) where
+  mem : set → set → Prop
+  emptyset : set
+  powerset : set → set
+  union : set → set → set
+  sUnion : set → set
+  inter : set → set → set
+  sInter : set → set
+  singleton : set → set
+  sprod : set → set → set
+  pair : set → set → set
+notation:50 x:50 " ∈' " S:50 => SetNotation.mem x S
+binder_predicate x " ∈' " y:term => `($x ∈' $y)
+notation:110 " 𝓟' " S:110 => SetNotation.powerset S
+notation " ∅' " => SetNotation.emptyset
+notation:65 S:65 " ∪' " T:65  => SetNotation.union S T
+notation:110 " ∪₀' " S:110  => SetNotation.sUnion S
+notation:65 S:65 " ∩' " T:65  => SetNotation.inter S T
+notation:110 " ∩₀' " S:110  => SetNotation.sInter S
+notation:150 "{" x "}'" => SetNotation.singleton x
+notation:82 S:82 " ×ˢ' " T:82 => SetNotation.sprod S T
+notation:150 "(" a:150 "," b:150 ")'" => SetNotation.pair a b
+
+def SetNotation.subset {set : Type u} [SetNotation set]
+  (S T : set) : Prop := ∀ x, x ∈' S → x ∈' T
+notation:50 S:50 " ⊆' " T:50 => SetNotation.subset S T
+binder_predicate x " ⊆' " y:term => `($x ∈' $y)
+
+def SetNotation.is_a_set {set : Type u} [SetNotation set]
+  (p : set → Prop) : Prop := ∃ s, ∀ x, x ∈' s ↔ p x
+export SetNotation (is_a_set)
+
+def exists_unique {α : Sort u} (p : α → Prop) : Prop := ∃ x, p x ∧ ∀ y, p y → y = x
+section
+open Lean
+open TSyntax.Compat
+macro "∃!" xs:explicitBinders ", " b:term : term => expandExplicitBinders ``exists_unique xs b
+end
+-- example of ∃! n : Nat, 0 < n < 2
+example : ∃! n : Nat, 0 < n ∧ n < 2 := by
+  unfold exists_unique
+  refine ⟨1, ?_, ?_⟩
+  . exact ⟨Nat.lt_add_one _, Nat.lt_add_one _⟩
+  . intro y hy
+    have h1 : 1 ≤ y := Nat.succ_le_of_lt hy.1
+    have h2 : y ≤ 1 := Nat.le_of_lt_succ hy.2
+    exact Nat.le_antisymm h2 h1
+
+
+def SetNotation.is_a_function {set : Type u} [SetNotation set]
+  (f A B : set) : Prop := f ⊆' A ×ˢ' B ∧ ∀ x ∈' A, ∃! y, (x, y)' ∈' f
+export SetNotation (is_a_function)
 
 -- Definition 14.1 (unfinished)
-structure ZF where
-  set : Type u
-  mem : set → set → Prop
-  extensionality : ∀ A B : set, A = B ↔ (∀ x, mem x A ↔ mem x B)
-  emptyset : ∃ S, ∀ x, ¬ mem x S
-  replacement :
-    ∀ (P : set → set → Prop)
-      (_ : ∀ x, ∃ y, (P x y ∧ (∀ z, P x z → z = y)))
-      (U : set),
-    ∃ U', ∀ y, mem y U' ↔ (∃ x, mem x U ∧ P x y)
-  powerset :
-    ∀ S, ∃ PS, ∀ T, mem T PS ↔ (∀ x, mem x T → mem x S)
+class ZFC (set : Type u) extends SetNotation set where
+  extensionality (A B : set) : A = B ↔ (∀ x, x ∈' A ↔ x ∈' B)
+  emptyset_def : ∀ x : set, ¬ x ∈' ∅'
+  replacement (P : set → set → Prop) (hP : ∀ x, ∃! y, P x y) :
+    ∀ U : set, is_a_set fun y ↦ ∃ x ∈' U, P x y
+  powerset_def (S : set) : ∀ T, T ∈' 𝓟' S ↔ T ⊆' S
+  union_def (S T : set) : ∀ x, x ∈' S ∪' T ↔ x ∈' S ∨ x ∈' T -- redundten
+  sUnion_def (S : set) : ∀ x, x ∈' ∪₀' S ↔ ∃ A ∈' S, x ∈' A
+  inter_def (S T : set) : ∀ x, x ∈' S ∩' T ↔ x ∈' S ∧ x ∈' T -- redundten
+  sInter_def (S : set) : ∀ x, x ∈' ∩₀' S ↔ ∀ A ∈' S, x ∈' A -- redundten
+  infinity : ∃ S : set, ∅' ∈' S ∧ ∀ x ∈' S, x ∪' {x}' ∈' S
+  regularity : ∀ S ≠ (∅' : set), ∃ A ∈' S, A ∩' S = ∅'
+  pair_def (a b : set) : (a,b)' = { {a}' }' ∪' { {a}' ∪' {b}' }' -- (a,b) = {{a},{a,b}}, redundten
+  sprod_def (A B : set) : ∀ x, x ∈' A ×ˢ' B ↔ ∃ a ∈' A, ∃ b ∈' B, x = (a, b)' -- redundten
+  choice (S : set) (hs : S ≠ ∅') :
+    ∃ f, is_a_function f S (𝓟' S) ∧ ∀ T, T ≠ ∅' → T ⊆' S → ∃ y ∈' T, (T, y)' ∈' f
 
 -- Proposition 15.1.2
-theorem pairing (zf : ZF) (a b : zf.set) :
-  ∃ S, ∀ x, zf.mem x S ↔ x = a ∨ x = b := by
+theorem pairing {set : Type u} [ZFC set] (a b : set) :
+  is_a_set fun x ↦ x = a ∨ x = b := by
   -- zero = ∅
-  let ⟨zero, hzero⟩ := zf.emptyset
+  let zero : set := ∅'
+  let hzero := ZFC.emptyset_def (set := set)
   -- one = {∅}
-  let ⟨one, hone⟩ := zf.powerset zero
-  have zero_mem_one : zf.mem zero one := by
+  let one := 𝓟' zero
+  let hone := ZFC.powerset_def zero
+  have zero_mem_one : zero ∈' one := by
     rw [hone]
     intro x hxzero
     exact (hzero x hxzero).elim
   -- two = {∅, {∅}}
-  let ⟨two, htwo⟩ := zf.powerset one
-  have zero_mem_two : zf.mem zero two := by
+  let two := 𝓟' one
+  let htwo := ZFC.powerset_def one
+  have zero_mem_two : zero ∈' two := by
     rw [htwo]
     intro x hxzero
     exact (hzero x hxzero).elim
-  have one_mem_two : zf.mem one two := by
+  have one_mem_two : one ∈' two := by
     rw [htwo]
     intro x hxzero
     exact hxzero
   have zero_ne_one : zero ≠ one := by
     intro h
-    rw [zf.extensionality] at h
+    rw [ZFC.extensionality] at h
     have := h zero
     exact hzero zero (this.mpr zero_mem_one)
   -- ∀ x, ∃! y, P x y
@@ -65,7 +124,7 @@ theorem pairing (zf : ZF) (a b : zf.set) :
         . exact fun h' ↦ (h h'.1).elim
         . exact fun h' ↦ h'.2
 
-  let ⟨S, hS⟩ := zf.replacement P hP two
+  let ⟨S, hS⟩ := ZFC.replacement P hP two
   refine ⟨S, ?_⟩
   intro y
   constructor
